src/MemoryBlockC.v
@@ -5,6 +5,7 @@ Require Import
   Here.Relations
   Here.Heap
   Here.HeapADT
+  Here.FMapExt
   Coq.FSets.FMapFacts
   Coq.Structures.DecidableTypeEx.
 
@@ -13,10 +14,10 @@ Module MemoryBlockC (Mem : Memory) (M : WSfun N_as_DT).
 Module Import Adt := HeapADT Mem.
 Import Heap.
 
-Module P := WProperties_fun N_as_DT M.
-Module F := P.F.
-
 Module Import FunMaps := FunMaps N_as_DT M.
+Import FunMaps.FMapExt.
+Module P := FunMaps.FMapExt.P.
+Module F := P.F.
 
 Definition MemoryBlock_Same (x y : MemoryBlock) : Prop :=
   memSize x = memSize y /\ Same (memData x) (memData y).
@@ -182,12 +183,35 @@ Proof. intros ?????; exists y; reflexivity. Qed.
 
 Hint Resolve TotalMapRelation_r_eq.
 
-Lemma of_mem_MemoryBlock_AbsR : forall x,
+Lemma of_map_MemoryBlock_AbsR : forall x,
   MemoryBlock_AbsR {| memSize := memCSize x
                     ; memData := of_map eq (memCData x) |} x.
 Proof. split; intros; auto; apply of_map_Map_AbsR; auto. Qed.
 
-Hint Resolve of_mem_MemoryBlock_AbsR.
+Hint Resolve of_map_MemoryBlock_AbsR.
+
+Lemma Lookup_of_map : forall addr cblk r_o r_n,
+  Map_AbsR MemoryBlock_AbsR r_o r_n
+    -> M.MapsTo addr cblk r_n
+    -> Lookup addr {| memSize := memCSize cblk
+                    ; memData := of_map eq (memCData cblk) |} r_o.
+Proof.
+  intros.
+  apply H in H0.
+  destruct H0, H0, H1.
+  apply of_map_Same in H2.
+  apply H.
+  exists cblk.
+  intuition.
+  apply H.
+  exists x.
+  intuition.
+  split; intros; trivial.
+  rewrite H2.
+  apply of_map_Map_AbsR; auto.
+Qed.
+
+Hint Resolve Lookup_of_map.
 
 Ltac swap_sizes :=
   match goal with
@@ -196,5 +220,95 @@ Ltac swap_sizes :=
   | [ H : MemoryBlock_AbsR ?blk ?cblk |- context [memCSize ?cblk] ] =>
     rewrite <- (proj1 H)
   end.
+
+Definition keep_keys (P : M.key -> bool) : M.t Mem.Word8 -> M.t Mem.Word8 :=
+  P.filter (const ∘ P).
+
+Definition shift_keys (orig_base : N) (new_base : N) (m : M.t Mem.Word8) :
+  M.t Mem.Word8 :=
+  M.fold (fun k => M.add (k - orig_base + new_base)) m (M.empty _).
+
+Lemma KeepKeys_Map_AbsR :
+  KeepKeys [R (N.eq ==> boolR) ==> Map_AbsR eq ==> Map_AbsR eq] keep_keys.
+Proof.
+  unfold KeepKeys, keep_keys, compose, const.
+  constructor.
+  intros ???.
+  apply Filter_Map_AbsR; auto; relational.
+  apply H; reflexivity.
+Qed.
+
+Lemma ShiftKeys_Map_AbsR : forall b d r m,
+  r [R Map_AbsR eq] m ->
+  All (fun k _ => b <= k) r ->
+  (* P.for_all (fun k _ => b <=? k) m -> *)
+  ShiftKeys b d r [R Map_AbsR eq] shift_keys b d m.
+Proof.
+  unfold ShiftKeys, shift_keys, compose, const; intros.
+  eapply (All_Map_AbsR (A:=Mem.Word8) (B:=Mem.Word8) (R:=eq)
+                       (f:=fun k _ => b <= k) (f':=fun k _ => b <=? k)) in H0.
+    Focus 2. relational.
+    Focus 2. relational. split; nomega.
+    Focus 2. apply logical_prf.
+  relational; split; intros; split; intros H1.
+  - repeat teardown.
+    inversion H1; subst; clear H1.
+    apply H in H2;
+    destruct H2 as [cblk [? ?]]; subst.
+    pose proof H0.
+    apply (proj1 (P.for_all_iff _ _)) with (k:=n) (e:=cblk) in H2; [|exact H1].
+    exists cblk; intuition.
+    revert H1.
+    revert H0.
+    apply P.fold_rec_bis; auto; intros.
+      rewrite <- H0 in H3, H4; intuition.
+    repeat simplify_maps.
+    apply for_all_add_true in H4;
+    destruct H4; auto; relational.
+    right; intuition.
+    apply N.add_cancel_r in H6.
+    apply Nsub_eq in H6; auto; nomega.
+  - reduction.
+    revert H1.
+    revert H0.
+    apply P.fold_rec_bis; auto; intros.
+      rewrite <- H0 in H2; intuition.
+    apply for_all_add_true in H3;
+    destruct H3; auto; relational.
+    simplify_maps.
+    exists (k, x); simpl.
+    apply H in H0; destruct H0.
+    intuition; subst; assumption.
+  - revert H1.
+    revert H0.
+    apply P.fold_rec_bis; auto; intros.
+      rewrite <- H0 in H2; intuition.
+    apply for_all_add_true in H3;
+    destruct H3; auto; relational.
+    simplify_maps.
+    exists cblk; simpl.
+    intuition.
+    pose proof (Lookup_Map_set (B:=Mem.Word8) (a:=k - b + d) (b:=cblk)
+                               (fun p => (fst p - b + d, snd p))).
+    apply H2.
+    exists (k, cblk); simpl.
+    apply H in H0; destruct H0.
+    intuition; subst; assumption.
+  - repeat teardown; subst.
+    inversion H1; subst; clear H1.
+    apply H in H3.
+    destruct H3 as [blk [? ?]]; subst.
+    revert H1.
+    revert H0.
+    apply P.fold_rec_bis; auto; intros.
+      rewrite <- H0 in H2, H3; intuition.
+    apply for_all_add_true in H3;
+    destruct H3; auto; relational.
+    repeat simplify_maps.
+    right; intuition.
+    apply (proj1 (P.for_all_iff _ _)) with (k0:=n) (e0:=blk) in H3; [|exact H9].
+    apply N.add_cancel_r in H4.
+    apply Nsub_eq in H4; auto; nomega.
+Qed.
 
 End MemoryBlockC.
