src/Pending.v
@@ -1,0 +1,126 @@
+(*
+Lemma keep_keys_fold : forall soff doff len s d,
+  M.Equal (M.fold (fun k e m =>
+                     if within_bool soff len k
+                     then M.add (k - soff + doff) e m
+                     else m) s d)
+          (M.fold (fun k => M.add (k - soff + doff))
+                  (keep_keys (within_bool soff len) s) d).
+
+Lemma keep_shift_fold : forall soff doff s d,
+  P.for_all (fun k _ => soff <=? k) s ->
+  M.Equal (M.fold (fun k => M.add (k - soff + doff)) s d)
+          (P.update d (shift_keys soff doff s)).
+Proof.
+  unfold P.update, shift_keys; intros.
+  revert H.
+  apply P.fold_rec; intros.
+    rewrite P.fold_Empty; auto.
+      reflexivity.
+    rewrite P.fold_Empty; auto.
+    apply M.empty_1.
+
+  apply add_equal_iff in H1.
+  rewrite <- H1 in H3.
+  apply for_all_add_true in H3;
+  destruct H3; auto; relational.
+  intuition.
+
+  assert (P.transpose_neqkey M.Equal (@M.add Mem.Word8)).
+    intros ??????.
+    apply add_associative; tauto.
+
+  assert (Proper (eq ==> eq ==> M.Equal ==> M.Equal) (@M.add Mem.Word8)).
+    relational.
+    rewrite <- H8.
+    reflexivity.
+
+  remember (fun _ => M.add _) as f.
+  assert (P.transpose_neqkey M.Equal f).
+    intros ??????.
+    rewrite Heqf.
+    apply add_associative; intros.
+    apply N.add_cancel_r in H8.
+    apply Nsub_eq in H8.
+        contradiction.
+      a d m i t.
+    a d m i t.
+
+  assert (Proper (eq ==> eq ==> M.Equal ==> M.Equal) f).
+    relational.
+    rewrite <- H10.
+    reflexivity.
+
+  pose proof (@fold_Proper Mem.Word8 _ (@M.add Mem.Word8) M.Equal
+                           (F.EqualSetoid _) H6 H2).
+  pose proof (@fold_Proper Mem.Word8 _ f M.Equal (F.EqualSetoid _) H8 H7).
+
+  rewrite <- H1.
+  apply add_equal_iff in H1.
+
+  erewrite P.fold_add; eauto.
+  rewrite H5, Heqf.
+  erewrite P.fold_add; eauto.
+    reflexivity.
+  unfold not; intros; destruct H11.
+  contradiction H0.
+  exists x.
+  revert H11.
+  apply P.fold_rec_bis; intros; auto.
+    rewrite <- H11.
+    intuition.
+  repeat simplify_maps.
+    left; intuition.
+    apply N.add_cancel_r in H15.
+    apply (proj1 (P.for_all_iff _ _)) with (k1:=k0) (e0:=x) in H3;
+    [|exact H11].
+    apply Nsub_eq in H15; auto; nomega.
+  right; intuition; subst; tauto.
+*)
+
+Lemma Map_set_fold_keys_AbsR : forall elt r (m : M.t elt) f,
+  (forall x y : M.key, E.eq (f x) (f y) -> E.eq x y)
+    -> r [R Map_AbsR eq] m
+    -> Map_set (fun p => (f (fst p), snd p)) r
+         [R Map_AbsR eq]
+         M.fold (fun k : M.key => M.add (f k)) m (M.empty elt).
+Proof.
+  intros.
+  relational; split; intros; split; intros H1.
+  - repeat teardown; inv H1.
+    apply H0 in H2;
+    destruct H2 as [cblk [? ?]]; subst.
+    exists cblk; intuition.
+    revert H1.
+    apply P.fold_rec_bis; auto; intros.
+      rewrite <- H1 in H3; intuition.
+    repeat simplify_maps.
+    right; intuition.
+    apply H in H4.
+  - reduction.
+    revert H1.
+    apply P.fold_rec_bis; auto; intros.
+    simplify_maps.
+    exists (k, x); simpl.
+    apply H0 in H1; destruct H1.
+    intuition; subst; assumption.
+  - revert H1.
+    apply P.fold_rec_bis; auto; intros.
+    simplify_maps.
+    exists cblk; simpl.
+    intuition.
+    pose proof (Lookup_Map_set (B:=elt) (a:=f k) (b:=cblk)
+                               (fun p => (f (fst p), snd p))).
+    apply H4.
+    exists (k, cblk); simpl.
+    apply H0 in H1; destruct H1.
+    intuition; subst; assumption.
+  - repeat teardown; subst; inv H1.
+    apply H0 in H3.
+    destruct H3 as [blk [? ?]]; subst.
+    revert H1.
+    apply P.fold_rec_bis; auto; intros.
+      rewrite <- H1 in H3; intuition.
+    repeat simplify_maps.
+    right; intuition.
+Qed.
